theories/compiler/compiler.v
@@ -51,7 +51,7 @@ Lemma compile_correct f2i f fn dins ins a:
   (∀ f' i', f2i !! f' = Some i' → ins !! i' = None ↔ f' ≠ f) →
   trefines (MS asm_module (initial_asm_state ins))
            (MS (imp_to_asm (dom _ ins) {[f]} f2i imp_module)
-               (initial_imp_to_asm_state imp_module (initial_imp_state (<[f := fn]> ∅)))).
+               (initial_imp_to_asm_state ∅ imp_module (initial_imp_state (<[f := fn]> ∅)))).
 Proof.
   unfold compile.
   move => /compiler_success_bind_success[?[/compiler_success_fmap_error_success ? /compiler_success_fmap_error_success?]].
